Integrating [path] and [nonreachable] was not a good idea. Revert.

bf/bf_Graph_reach_nonneg_1.v
@@ -113,23 +113,28 @@ Axiom edges_def : forall (x:vertex) (y:vertex), (mem (x, y) edges) -> ((mem x
   vertices) /\ (mem y vertices)).
 
 (* Why3 assumption *)
-Inductive path : vertex -> vertex -> Z -> Z -> Prop :=
-  | path_empty : forall (v:vertex), (path v v 0%Z 0%Z)
-  | path_succ : forall (v1:vertex) (v2:vertex) (v3:vertex) (n:Z) (d:Z),
-      (path v1 v2 n d) -> ((mem (v2, v3) edges) -> (path v1 v3
-      (n + (weight v2 v3))%Z (d + 1%Z)%Z)).
+Inductive path : vertex -> vertex -> Z -> Prop :=
+  | path_empty : forall (v:vertex), (path v v 0%Z)
+  | path_succ : forall (v1:vertex) (v2:vertex) (v3:vertex) (n:Z), (path v1 v2
+      n) -> ((mem (v2, v3) edges) -> (path v1 v3 (n + (weight v2 v3))%Z)).
 
 (* Why3 assumption *)
-Definition shortest_path(v1:vertex) (v2:vertex) (n:Z): Prop := (exists d:Z,
-  (path v1 v2 n d)) /\ forall (m:Z) (d:Z), (m <  n)%Z -> ~ (path v1 v2 m d).
+Inductive reachable : vertex -> Z -> Prop :=
+  | reachable_empty : (reachable s 0%Z)
+  | reachable_succ : forall (v1:vertex) (v2:vertex) (d:Z), (reachable v1
+      d) -> ((mem (v1, v2) edges) -> (reachable v2 (d + 1%Z)%Z)).
 
 (* Why3 assumption *)
-Definition no_path(v1:vertex) (v2:vertex): Prop := forall (n:Z) (d:Z),
-  ~ (path v1 v2 n d).
+Definition shortest_path(v1:vertex) (v2:vertex) (n:Z): Prop := (path v1 v2
+  n) /\ forall (m:Z), (m <  n)%Z -> ~ (path v1 v2 m).
+
+(* Why3 assumption *)
+Definition no_path(v1:vertex) (v2:vertex): Prop := forall (n:Z), ~ (path v1
+  v2 n).
 
 (* Why3 goal *)
-Theorem path_depth_nonneg : forall (v1:vertex) (v2:vertex) (n:Z) (d:Z),
-  (path v1 v2 n d) -> (0%Z <= d)%Z.
+Theorem reach_nonneg : forall (v:vertex) (d:Z), (reachable v d) ->
+  (0%Z <= d)%Z.
 
 induction 1 ; omega.
 
